

5.3A.

31.(1) $\ln \sqrt{x^2+y^2} = \arctan \frac{y}{x}$

$F(x,y) = \ln \sqrt{x^2+y^2} - \arctan \frac{y}{x} = 0$

$F_x = \frac{x-y}{x^2+y^2}$

$F_y = \frac{y-x}{x^2+y^2}$

$\frac{dy}{dx} = -\frac{F_x}{F_y} = \frac{x+y}{x-y}$

$\frac{d^2y}{dx^2} = \frac{2x^2-2y^2}{(x-y)^3}$

32.(2) $x^2-2y^2+z^2-4x+2z-5=0$

$F(x,y,z) = x^2-2y^2+z^2-4x+2z-5=0$

$F_x = 2x-4$ $F_y = -4y$ $F_z = 2z+2$

$\frac{\partial z}{\partial x} = -\frac{F_x}{F_z} = \frac{x-2}{z+1}$ $\frac{\partial z}{\partial y} = -\frac{F_y}{F_z} = \frac{2y}{z+1}$

$\frac{\partial^2 z}{\partial x^2} = \frac{\partial}{\partial x} \left(\frac{\partial z}{\partial x} \right) = \frac{-(z+1)^2 - (x-2)^2}{(z+1)^3}$

$\frac{\partial^2 z}{\partial y^2} = \frac{\partial}{\partial y} \left(\frac{\partial z}{\partial y} \right) = \frac{2(z+1)^2 - 4y^2}{(z+1)^3}$

$\frac{\partial^2 z}{\partial x \partial y} = \frac{\partial}{\partial x} \left(\frac{\partial z}{\partial y} \right) = \frac{2y(x-2)}{(z+1)^3}$

$\frac{\partial^2 z}{\partial y \partial x} = \frac{\partial}{\partial y} \left(\frac{\partial z}{\partial x} \right) = \frac{2y(x-2)}{(z+1)^3}$

36.(2) $x^2+y^2+z^2 = y f\left(\frac{z}{y}\right)$

$F_x = x^2+y^2+z^2 - y f\left(\frac{z}{y}\right)$

$\frac{\partial z}{\partial x} = -\frac{F_x}{F_z} = \frac{2x}{y f'\left(\frac{z}{y}\right) - 2z}$

$\frac{\partial z}{\partial y} = -\frac{F_y}{F_z} = \frac{2y - f\left(\frac{z}{y}\right) + \frac{z}{y} f'\left(\frac{z}{y}\right)}{y f'\left(\frac{z}{y}\right) - 2z}$

$dz = \frac{\partial z}{\partial x} dx + \frac{\partial z}{\partial y} dy$

$= \frac{2x}{y f'\left(\frac{z}{y}\right) - 2z} dx + \frac{2y - f\left(\frac{z}{y}\right) + \frac{z}{y} f'\left(\frac{z}{y}\right)}{y f'\left(\frac{z}{y}\right) - 2z} dy$